[wip]

Clear/EVMState.lean
@@ -1,8 +1,13 @@
 import Mathlib.Data.Finmap
 import Mathlib.Data.Fin.Basic
+import Mathlib.Data.List.Intervals
 import Clear.Ast
 import Clear.Instr
 import Clear.UInt256
+import Clear.Wheels
+
+set_option linter.setOption false
+set_option pp.coercions false
 
 open Clear Instr UInt256
 
@@ -171,28 +176,162 @@ instance : Inhabited MachineState := ⟨ MachineState.mk ∅ 0 0 [] ⟩
 
 -- @langfield: Nit, but definitions should be camelCase.
 
-def UInt256.offsets : List UInt256 :=
+def UInt256.offsets : List ℕ :=
   [0,1,2,3,4,5,6,7,8,9,10,11,12,13,14,15,16,
   17,18,19,20,21,22,23,24,25,26,27,28,29,30,31]
 
+lemma UInt256.offsets_def : offsets = List.range 32 := by
+  repeat rw [ List.range_succ_eq_map ]
+  unfold offsets
+  simp
+
+lemma max_of_offsets_lt_32 : offsets.maximum < 32 := by decide
+lemma min_of_offsets_eq_0 : offsets.minimum = 0 := by decide
+
+lemma mem_offsets : ∀ {n}, n ∈ offsets ↔ n < 32 := by
+  intro n
+  rw [offsets_def]
+  simp
+
+@[simp]
+lemma mem_offsets_of_le_32 : ∀ {n}, n < 32 → n ∈ offsets :=
+  mem_offsets.mpr
+
+lemma le_32_of_mem_offsets : ∀ {n}, n ∈ offsets → n < 32 :=
+  mem_offsets.mp
+
+-- List.Ico not yet in mathlib
+lemma UInt256.offsets_eq_Ico : offsets = List.Ico 0 32 := by
+  unfold List.Ico
+  rw [ List.range'_eq_map_range, offsets_def ]
+  simp
+
+-- lemma UInt256.offsets_at_addr :
+--   ∀ (addr : UInt256),
+--   offsets.map (addr + ↑·) = List.Ico addr.val (addr.val + 32) := by
+--   intro addr
+--   rw [offsets_eq_Ico, List.Ico.map_add 0 32 addr, zero_add, add_comm]
+
+lemma UInt256.mem_offsets_iff_mem_Ico : ∀ {n}, n ∈ offsets ↔ n ∈ Set.Ico 0 32 := by
+  intro n
+  apply Iff.intro
+  · intro mem
+    simp
+    exact mem_offsets.mp mem
+  · intro mem
+    simp at mem
+    exact mem_offsets.mpr mem
+
+lemma UInt256.offsetted_addresses (addr : UInt256) : ∀ {n},
+  (h : n ∈ offsets) → addr + ↑n ∈ offsets.map (addr + ↑·) := by
+  intro n h
+  exact List.mem_map_of_mem (addr + ↑·) h
+
+-- lemma UInt256.word_addresses (addr : UInt256) :
+--   Set.MapsTo (addr + ↑·) (Set.Ico 0 32) (Set.Ico addr (addr + 32)) := by
+--   have : (addr + ↑·) '' (Set.Ico 0 32) = Set.Ico addr (addr + 32) := by
+--     dsimp [Set.image]
+--     conv => rhs; rw [← Set.Ico_def]
+    
+--     sorry
+    
+--   rw [← this]
+--   exact Set.mapsTo_image (addr + ↑·) (Set.Ico 0 32)
+  
+
+-- lemma UInt256.same_address_of_offsetted_addresses (addr addr': UInt256) {n} :
+--   (h : n ∈ offsets) →
+--   addr' + ↑n ∈ offsets.map (addr + ↑·) →
+--   addr' = addr := by
+--   intro h mem
+--   simp at mem
+--   sorry
+
+lemma UInt256.addresses_of (addr : UInt256) {a} :
+  a ∈ offsets.map (addr + ↑·) ↔ a ∈ Set.Ico addr (addr + 32) := by
+  sorry
+
+namespace UInt256
+
+def range' {n} (start : UInt256) (len : Fin (n + 1)) (step : UInt256 := 1) : List UInt256 :=
+  match start, len with
+  | _, 0 => []
+  | s, ⟨n+1, _⟩ => s :: range' (s + step) ⟨n, by linarith⟩ step
+
+@[simp]
+lemma range'_zero {s step : UInt256} : range' (n := 0) s 0 step = [] := by
+  unfold range'
+  rfl
+
+@[simp]
+lemma range'_one {s step : UInt256} : range' (n := 1) s 1 step = [s] := by
+  unfold range'
+  simp
+
+lemma range'_succ {n} (start : UInt256) (len : Fin (n + 2)) (step : UInt256) [NeZero len] :
+  range' start len step =
+    start :: range' (start + step) (len.pred NeZero.out) step := by
+  have ne : len ≠ 0 := NeZero.out
+  obtain ⟨y, y_succ_eq_len⟩ := Fin.exists_succ_eq_of_ne_zero ne
+  simp_rw [← y_succ_eq_len]
+  conv =>
+    lhs
+    unfold range'
+    simp
+    dsimp [Fin.succ]
+    
+  simp
+
+
+-- lemma range'_eq_cons_iff
+--   {s n a : UInt256} {xs : List UInt256} :
+--   range' s n = a :: xs ↔
+--     s = a ∧ 0 < n ∧ xs = range' (a + 1) (n - 1) := sorry
+
+lemma map_add_range' (a) : ∀ s n step,
+  List.map (λ (x : UInt256) ↦ a + x) (range' s n step) =
+    range' (a + s) n step
+  | _, 0, _ => by simp
+  | s, ⟨n+1, _⟩, step => sorry
+
+end UInt256
+
+lemma splice_toBytes! (v : UInt256) : toBytes! v = 
+  [ (toBytes! v)[0],   (toBytes! v)[1],   (toBytes! v)[2],   (toBytes! v)[3]
+  , (toBytes! v)[4],   (toBytes! v)[5],   (toBytes! v)[6],   (toBytes! v)[7]
+  , (toBytes! v)[8],   (toBytes! v)[9],   (toBytes! v)[10],  (toBytes! v)[11]
+  , (toBytes! v)[12],  (toBytes! v)[13],  (toBytes! v)[14],  (toBytes! v)[15]
+  , (toBytes! v)[16],  (toBytes! v)[17],  (toBytes! v)[18],  (toBytes! v)[19]
+  , (toBytes! v)[20],  (toBytes! v)[21],  (toBytes! v)[22],  (toBytes! v)[23]
+  , (toBytes! v)[24],  (toBytes! v)[25],  (toBytes! v)[26],  (toBytes! v)[27]
+  , (toBytes! v)[28],  (toBytes! v)[29],  (toBytes! v)[30],  (toBytes! v)[31]
+  ] := by
+  apply List.ext_get
+  · simp
+  · intro n h₁ h₂
+    simp at h₂
+    have h_offset := mem_offsets_of_le_32 h₂
+    fin_cases h_offset
+    all_goals aesop
+
 def MachineState.updateMemory (m : MachineState) (addr v : UInt256) : MachineState :=
-  {m with memory := let offsets := List.range 32
-                    let addrs   := offsets.map (·+addr)
+  {m with memory := let addrs   := offsets.map (addr + ↑·)
                     let inserts := addrs.zipWith Finmap.insert (UInt256.toBytes! v)
                     inserts.foldl (init := m.memory) (flip id)
           max_address := max addr m.max_address }
 
-lemma cheeky_proof {a b : Int} : (if a > b then a else b) = max a b := by rw [max_comm, max_def_lt]
+def MachineState.lookupByte (m : MachineState) (addr : UInt256) : UInt8 :=
+  (m.memory.lookup addr).get!
 
-def MachineState.lookupMemory (m : MachineState) (addr : UInt256) : UInt256 :=
-  UInt256.fromBytes! (List.map (fun i => (m.memory.lookup (addr + i)).get!) UInt256.offsets)
+def MachineState.lookupWord (m : MachineState) (addr : UInt256) : UInt256 :=
+--  UInt256.fromBytes! (offsets.map λ i ↦ (m.memory.lookup (addr + i)).get!)
+  UInt256.fromBytes! $ offsets.map $ m.lookupByte ∘ (addr + ↑·)
 
 def MachineState.setReturnData (m : MachineState) (r : List UInt256) : MachineState :=
   {m with return_data := r}
 
 def MachineState.msize (m : MachineState) : UInt256 :=
   m.max_address
-
 
 -- definition of the blocks
 
@@ -254,6 +393,11 @@ instance : Inhabited EVMState :=
 
 abbrev EVM := EVMState
 
+def preserved : EVMState → EVMState → Prop :=
+  (Eq on EVMState.account_map) ∩
+  (Eq on EVMState.hash_collision) ∩
+  (Eq on EVMState.execution_env)
+
 -- functions for querying balance
 
 namespace EVMState
@@ -263,7 +407,12 @@ section
 open Array ByteArray
 
 -- | Add an error to the EVMState indicating that we hit a hash collision in `keccak256`.
-def addHashCollision (σ : EVMState) : EVMState := { σ with hash_collision := True }
+def addHashCollision (σ : EVMState) : EVMState := { σ with hash_collision := true }
+
+-- def hasHashCollision (σ : EVMState) : Prop := σ.hash_collision = true
+
+-- instance : DecidablePred hasHashCollision := λ σ ↦
+--   decidable_of_bool σ.hash_collision (by unfold hasHashCollision; simp)
 
 def lookupAccount (σ : EVMState) (addr : Address) : Option Account :=
   σ.account_map.lookup addr
@@ -296,8 +445,8 @@ def calldatacopy (σ : EVMState) (mstart datastart s : UInt256) : EVMState :=
 def mkInterval (ms : MachineState) (p n : UInt256) : List UInt256 :=
   let i : ℕ := p.val
   let f : ℕ := n.val
-  let m     := (List.range' i f).map Fin.ofNat
-  m.map ms.lookupMemory
+  let m     := (List.range' i f 32).map Fin.ofNat
+  m.map ms.lookupWord
 
 def keccak256 (σ : EVMState) (p n : UInt256) : Option (UInt256 × EVMState) :=
   let interval : List UInt256 := mkInterval σ.machine_state p n
@@ -381,7 +530,7 @@ def selfbalance (σ : EVMState) : UInt256 :=
 -- memory and storage operations
 
 def mload (σ : EVMState) (spos : UInt256) : UInt256 :=
-  σ.machine_state.lookupMemory spos
+  σ.machine_state.lookupWord spos
 
 def mstore (σ : EVMState) (spos sval : UInt256) : EVMState :=
   σ.updateMemory spos sval
@@ -431,5 +580,207 @@ def evm_revert (σ : EVMState) (mstart s : UInt256) : EVMState :=
   σ.evm_return mstart s
 
 end
+
+section Memory
+
+section MachineState
+
+variable {p n : UInt256}
+variable {ms : MachineState}
+variable {val : UInt256}
+
+lemma lt_toBytes_length_of_mem_offset :
+  ∀ {offset}, (v : UInt256) → (offset ∈ offsets) → offset < (toBytes! v).length := by
+  unfold offsets
+  simp
+  
+lemma lookupBytes_nil :
+  ∀ {addr},
+  [].map (ms.lookupByte ∘ (addr + ↑·)) = [] := by
+  simp
+
+lemma lookupBytes_cons :
+  ∀ {addr} {offset : ℕ} {os : List ℕ},
+  (offset :: os).map ((ms.updateMemory addr val).lookupByte ∘ (addr + ↑·)) = 
+    (ms.updateMemory addr val).lookupByte (addr + ↑offset)
+    :: os.map ((ms.updateMemory addr val).lookupByte ∘ (addr + ↑·)) := by
+  intro addr offset os
+  exact List.map_cons
+    ((ms.updateMemory addr val).lookupByte ∘ (addr + ↑·))
+    offset
+    os
+
+-- TODO: in newer mathlib
+@[simp] theorem get!_some {α} [Inhabited α] {a : α} : (some a).get! = a := rfl
+
+lemma lookupByte_updateMemory :
+  ∀ {addr},
+  (ms.updateMemory addr val).lookupByte addr =
+    (UInt256.toBytes! val)[0] := by
+  intro addr
+  unfold MachineState.updateMemory MachineState.lookupByte
+  simp
+  rw [ List.zipWith_foldl_eq_zip_foldl ]
+  conv => lhs; rw [splice_toBytes! val]
+  unfold offsets
+  simp only [List.map, List.zip, List.zipWith, List.foldl, flip, id]
+  norm_cast
+  rw [ Fin.add_zero addr ]
+  simp
+
+lemma lookupByte_updateMemory_of_ne :
+  ∀ {addr addr' : UInt256},
+  (h : addr' ∉ offsets.map (addr + ↑·)) →
+  (ms.updateMemory addr val).lookupByte addr' =
+    ms.lookupByte addr' := by
+  intro addr addr' h
+  unfold MachineState.updateMemory MachineState.lookupByte
+  simp
+  rw [ List.zipWith_foldl_eq_zip_foldl ]
+  conv => lhs; rw [splice_toBytes! val]
+  unfold offsets
+  simp only [List.map, List.zip, List.zipWith, List.foldl, flip, id]
+  norm_cast
+  rw [ Fin.add_zero addr ]
+  
+  unfold offsets at h
+  simp at h
+  repeat rw [← ne_eq] at h
+  let ⟨_,_,_,_,_,_,_,_,_,_,_,_,_,_,_,_,_,_,_,_,_,_,_,_,_,_,_,_,_,_,_,_⟩ := h
+
+  rw [ Finmap.lookup_insert_of_ne, Finmap.lookup_insert_of_ne, Finmap.lookup_insert_of_ne
+     , Finmap.lookup_insert_of_ne, Finmap.lookup_insert_of_ne, Finmap.lookup_insert_of_ne
+     , Finmap.lookup_insert_of_ne, Finmap.lookup_insert_of_ne, Finmap.lookup_insert_of_ne
+     , Finmap.lookup_insert_of_ne, Finmap.lookup_insert_of_ne, Finmap.lookup_insert_of_ne
+     , Finmap.lookup_insert_of_ne, Finmap.lookup_insert_of_ne, Finmap.lookup_insert_of_ne
+     , Finmap.lookup_insert_of_ne, Finmap.lookup_insert_of_ne, Finmap.lookup_insert_of_ne
+     , Finmap.lookup_insert_of_ne, Finmap.lookup_insert_of_ne, Finmap.lookup_insert_of_ne
+     , Finmap.lookup_insert_of_ne, Finmap.lookup_insert_of_ne, Finmap.lookup_insert_of_ne
+     , Finmap.lookup_insert_of_ne, Finmap.lookup_insert_of_ne, Finmap.lookup_insert_of_ne
+     , Finmap.lookup_insert_of_ne, Finmap.lookup_insert_of_ne, Finmap.lookup_insert_of_ne
+     , Finmap.lookup_insert_of_ne, Finmap.lookup_insert_of_ne
+     ]
+
+  all_goals assumption
+
+lemma lookupByte_at_offset_updateMemory :
+  ∀ {addr} {n}, (mem: n ∈ offsets) →
+  (ms.updateMemory addr val).lookupByte (addr + ↑n) =
+    (UInt256.toBytes! val)[n]'(lt_toBytes_length_of_mem_offset val mem) := by
+  intro addr n mem
+  unfold MachineState.updateMemory MachineState.lookupByte
+  simp
+  rw [ List.zipWith_foldl_eq_zip_foldl ]
+  conv => lhs; rw [splice_toBytes! val]
+  unfold offsets
+  simp only [List.map, List.zip, List.zipWith, List.foldl, flip, id]
+  norm_cast
+  fin_cases mem
+  · rw [ Nat.cast_zero, Fin.add_zero addr ]
+    simp
+  · rw [ Nat.cast_one ]
+    simp
+  all_goals simp only [ Nat.cast_ofNat, Fin.isValue, List.getElem_eq_get, add_zero, ne_eq
+                      , add_right_inj, Fin.reduceEq, not_false_eq_true
+                      , Finmap.lookup_insert_of_ne, Finmap.lookup_insert, get!_some
+                      ]
+
+lemma lookupByte_at_offset_updateMemory_of_ne {addr addr' : UInt256} :
+  ∀ {n}, (mem: n ∈ offsets) →
+  (h : addr' + ↑n ∉ offsets.map (addr + ↑·)) →
+  (ms.updateMemory addr val).lookupByte (addr' + ↑n) =
+    ms.lookupByte (addr' + ↑n) := by
+  intro n mem h
+  apply lookupByte_updateMemory_of_ne (addr' := addr' + ↑n)
+  assumption
+
+lemma lookupWord_updateMemory : ∀ {addr}, (ms.updateMemory addr val).lookupWord addr = val := by
+  intro addr
+  unfold MachineState.lookupWord offsets
+  repeat rw [ lookupBytes_cons, lookupByte_at_offset_updateMemory (by simp) ]
+  rw [ List.map_nil
+     , ← splice_toBytes!
+     , fromBytes!_toBytes!
+     ]
+
+-- set_option maxHeartbeats 5000000
+
+lemma lookupWord_updateMemory_of_ne {addr addr' : UInt256} :
+  ∀ {n}, (mem: n ∈ offsets) →
+  (h : addr' + ↑n ∉ offsets.map (addr + ↑·)) →
+  (ms.updateMemory addr val).lookupWord addr' = ms.lookupWord addr' := by
+  intro n mem h
+    
+  unfold MachineState.lookupWord
+  
+  rw [ ← List.map_comp_map
+     , Function.comp_apply
+     , ← List.map_comp_map
+     , Function.comp_apply
+     -- , Function.comp_def
+     ]
+  sorry
+
+-- lemma updateMemory_updateMemory :
+--   ∀ {addr} {val val'},
+--   (ms.updateMemory addr val).updateMemory addr val' = ms.updateMemory addr val' := by
+--   sorry
+
+end MachineState
+
+section Interval
+
+variable {p n : UInt256}
+variable {evm : EVM}
+variable {ms : MachineState}
+variable {val : UInt256}
+
+  -- mkInterval (mstore evm x v) x = v :: (mkInterval evm (x + 32))
+
+lemma zero_len_eq_nil :
+  mkInterval ms p 0 = [] := by
+  unfold mkInterval
+  simp
+
+theorem List.range'_succ (s n step) :
+  List.range' s (n + 1) step = s :: List.range' (s + step) n step := by
+  simp [List.range', Nat.add_succ, Nat.mul_succ]
+
+lemma ofNat_of_val (k : UInt256) : (Fin.ofNat k.val : UInt256) = k := by
+  dsimp [Fin.ofNat]
+  simp_rw [ ← UInt256.size_def, Nat.mod_eq_of_lt k.isLt ]
+  rfl
+
+lemma succ_len_eq_cons [NeZero n] :
+  mkInterval (mstore evm p val).machine_state p n =
+    val :: mkInterval evm.machine_state (p + 1) (n - 1) := by
+  -- generalize k_def : n.pred h = k
+  -- have k : UInt256 := n.pred h
+  have ne : n.val ≠ 0 := Fin.val_ne_of_ne NeZero.out
+  have one_le_n : 1 ≤ n.val := Nat.one_le_iff_ne_zero.mpr ne
+  have u_def : Σ' u : ℕ, u.succ = ↑n := by
+    use (n.pred NeZero.out).val
+    simp
+    rw [Nat.sub_add_cancel one_le_n]
+
+  let ⟨u, succ_u_eq_n⟩ := u_def
+  
+  unfold mstore mkInterval updateMemory
+  simp
+  rw [ ← succ_u_eq_n, List.range'_succ ↑p ↑u 1, List.map_cons ]
+  rw [Function.comp_apply] -- dsimp [(· ∘ ·)]
+
+  have u_eq_pred_n : u = n - 1 := by
+    rw [← Nat.succ_inj]
+    dsimp
+    rw [Nat.sub_add_cancel one_le_n]
+    exact succ_u_eq_n
+
+  rw [ ofNat_of_val p, @lookupWord_updateMemory evm.machine_state val p ]
+  rw [ u_eq_pred_n ]
+  simp
+  sorry
+
+end Memory.Interval
 
 end Clear.EVMState
