Generated/erc20shim/ERC20Shim/Predicate.lean
@@ -1,0 +1,67 @@
+import Mathlib.Data.Finmap
+
+import Clear.State
+
+import Generated.erc20shim.ERC20Shim.Variables
+
+open Clear
+
+namespace Generated.erc20shim.ERC20Shim
+
+abbrev BalanceMap := Finmap (λ _ : Address ↦ UInt256)
+abbrev AllowanceMap := Finmap (λ _ : Address × Address ↦ UInt256)
+
+structure ERC20 where
+  supply : UInt256
+  balances : BalanceMap
+  allowances : AllowanceMap
+
+-- structure HasBalance (balances : BalanceMap) (account : Address) (s : State) where
+--   address : Address
+--   keccak : s.evm.keccak_map.lookup [ ↑account , ERC20Private.balances ] = some address
+--   balance : some (s.evm.sload address) = balances.lookup account
+
+abbrev HasBalance (balances : BalanceMap) (account : Address) (s : State) :=
+  ∃ address,
+  s.evm.keccak_map.lookup [ ↑account , ERC20Private.balances ] = some address ∧
+  some (s.evm.sload address) = balances.lookup account
+
+namespace HasBalance
+
+variable {balances : BalanceMap} {account : Address} {s : State}
+
+-- theorem keccak (address(h : HasBalance balances account s) :
+--   ∃ address, s.evm.keccak_map.lookup [ ↑account , ERC20Private.balances ] = some address := 
+--   let ⟨addr, keccak, _⟩ := h
+--   ⟨addr, keccak⟩
+
+-- theorem balance (h : HasBalance balances account s) :
+--   ∃ address, some (s.evm.sload address) = balances.lookup account :=
+--   let ⟨addr, _, balance⟩ := h
+--   ⟨addr, balance⟩
+
+end HasBalance
+
+-- structure HasAllowance (allowances : AllowanceMap) (owner : Address) (spender : Address) (s : State) where
+--   address : Address
+--   keccak : s.evm.keccak_map.lookup [ ↑owner, ↑spender, ERC20Private.allowances ] = some address
+--   allowance : some (s.evm.sload address) = allowances.lookup ⟨owner, spender⟩
+
+def HasAllowance (allowances : AllowanceMap) (owner : Address) (spender : Address) (s : State) : Prop :=
+  ∃ address,
+  s.evm.keccak_map.lookup [ ↑owner, ↑spender, ERC20Private.allowances ] = some address ∧
+  some (s.evm.sload address) = allowances.lookup ⟨owner, spender⟩
+
+-- def balance_predicate (erc20 : ERC20) (s : State) : Prop :=
+--   ∀ account,
+--   account ∈ erc20.balances → HasBalance erc20.balances account s
+
+-- def balance_predicate (erc20 : ERC20) (s : State) : ? :=
+--   ∀ account,
+--   account ∈ erc20.balances → HasBalance erc20.balances account s
+
+def allowance_predicate (erc20 : ERC20) (s : State) : Prop :=
+  ∀ (owner spender : Address),
+  ⟨owner, spender⟩ ∈ erc20.allowances → HasAllowance erc20.allowances owner spender s
+
+end Generated.erc20shim.ERC20Shim
