Generated/erc20shim/ERC20Shim/Variables.lean
@@ -1,4 +1,10 @@
+import Mathlib.Data.Finmap
+import Clear.Ast
+import Clear.EVMState
 import Clear.UInt256
+import Clear.State
+
+open Clear
 
 namespace Generated.erc20shim.ERC20Shim
 
@@ -11,5 +17,11 @@ structure PrivateAddresses where
 
 def ERC20Private : PrivateAddresses :=
   { balances := 0, allowances := 1, totalSupply := 2, name := 3, symbol := 4 }
+
+
+def ERC20Pred (balances : Finmap (λ (_ : Address) ↦ UInt256)) (s : State) : Prop :=
+  ∀ account, account ∈ balances →
+  ∃ addr, s.evm.keccak_map.lookup [ ↑account , ERC20Private.balances ] = some addr ∧
+  some (s.evm.sload addr) = balances.lookup account
 
 end Generated.erc20shim.ERC20Shim
