Generated/erc20shim/ERC20Shim/fun_balanceOf_user.lean
@@ -1,9 +1,9 @@
 import Clear.ReasoningPrinciple
 
-import Generated.erc20shim.ERC20Shim.mapping_index_access_mapping_address_uint256_of_address
-
+-- import Generated.erc20shim.ERC20Shim.mapping_index_access_mapping_address_uint256_of_address
 import Generated.erc20shim.ERC20Shim.fun_balanceOf_gen
 
+import Generated.erc20shim.ERC20Shim.Predicate
 
 namespace Generated.erc20shim.ERC20Shim
 
@@ -11,13 +11,42 @@ section
 
 open Clear EVMState Ast Expr Stmt FunctionDefinition State Interpreter ExecLemmas OutOfFuelLemmas Abstraction YulNotation PrimOps ReasoningPrinciple Utilities Generated.erc20shim ERC20Shim
 
-def A_fun_balanceOf (var : Identifier) (var_account : Literal) (s₀ s₉ : State) : Prop := sorry
+def A_fun_balanceOf (var : Identifier) (var_account : Literal) (s₀ s₉ : State) : Prop :=
+  ∀ erc20, balance_predicate erc20 s₀ → balance_predicate erc20 s₉
+
+  -- ∃ (s : State) (addr : UInt256), (s₉ = s⟦ var ↦ s.evm.sload addr ⟧)
 
 lemma fun_balanceOf_abs_of_concrete {s₀ s₉ : State} {var var_account} :
   Spec (fun_balanceOf_concrete_of_code.1 var var_account) s₀ s₉ →
   Spec (A_fun_balanceOf var var_account) s₀ s₉ := by
-  unfold fun_balanceOf_concrete_of_code A_fun_balanceOf
-  sorry
+  unfold fun_balanceOf_concrete_of_code A_fun_balanceOf  
+  rcases s₀ with ⟨evm, varstore⟩ | _ | _ <;> [simp only; aesop_spec; aesop_spec]
+  apply spec_eq
+  clr_funargs
+
+  intro hasFuel index_access erc20 pred_s₀
+
+  rcases index_access with ⟨sₖ, mapping, h'⟩
+  -- clr_spec at mapping
+
+  -- have sₖ_isOk : isOk sₖ := mapping_of_ok mapping (by simp)
+  -- rcases sₖ with ⟨evmₖ, _⟩ | _ | _ <;> try contradiction
+  -- use (Ok evmₖ varstore)
+
+  -- simp at *
+  -- rw [ ← State.insert_of_ok, ← State.insert_of_ok
+  --    , State.lookup_insert
+  --    ] at h'
+  -- symm at h'
+
+  -- by_cases h : evmₖ.hash_collision = true
+  -- · use 0
+  --   rw [ lookup_addr_fail mapping h] at h'
+  --   assumption
+  -- · rcases lookup_addr_ok mapping (by aesop) with ⟨addr, lookup_eq_addr⟩
+  --   use addr
+  --   rw [ lookup_eq_addr ] at h'
+  --   assumption
 
 end
 
